change narrowing to use inductive subenvironment

src/simple-proof/proof/Narrowing.v
@@ -9,16 +9,30 @@ Set Implicit Arguments.
 Require Import LibLN.
 Require Import Definitions.
 Require Import Weakening.
+Require Import Coq.Program.Equality.
 
 
 (** [G1] is a subenvironment of [G2], denoted [G1 subG G2],
      if for each [x] s.t. [G2(x)=T2],
     [G1(x) = T1] and [G1 ⊢ T1 <: T2]. *)
-Definition subenv(G1 G2: ctx) :=
-  forall x T2, binds x T2 G2 ->
-    binds x T2 G1 \/
-    exists T1,
-      binds x T1 G1 /\ G1 ⊢ T1 <: T2.
+Reserved Notation "G1 ⪯ G2" (at level 35).
+Inductive subenv: ctx -> ctx -> Prop :=
+| subenv_empty : empty ⪯ empty
+| subenv_grow: forall G G' x T T',
+    G ⪯ G' ->
+    ok (G & x ~ T) ->
+    ok (G' & x ~ T') ->
+    G ⊢ T <: T' ->
+    G & x ~ T ⪯ G' & x ~ T'
+where "G1 ⪯ G2" := (subenv G1 G2).
+Hint Constructors subenv.
+
+Lemma subenv_refl : forall G, ok G -> G ⪯ G.
+Proof.
+  intros G H. induction H; auto.
+Qed.
+Hint Resolve subenv_refl.
+
 
 (** [G' subG G]              #<br>#
     [ok(G', x: T)]               #<br>#
@@ -26,22 +40,15 @@ Definition subenv(G1 G2: ctx) :=
     [G', x: T subG G, x: T]  #<br>#
     Note: [ok(G)] means that [G]'s domain consists of distinct variables.
     [ok] is defined in [TLC.LibEnv.v]. *)
-Lemma subenv_push: forall G G' x T,
-  subenv G' G ->
-  ok (G' & x ~ T) ->
-  subenv (G' & x ~ T) (G & x ~ T).
+Lemma subenv_push : forall G1 G2 x T,
+    G1 ⪯ G2 ->
+    ok (G1 & x ~ T) -> ok (G2 & x ~ T) ->
+    (G1 & x ~ T) ⪯ (G2 & x ~ T).
 Proof.
-  intros.
-  unfold subenv. intros xb Tb Bi. apply binds_push_inv in Bi.
-  destruct Bi as [Bi | Bi].
-  + destruct Bi as [Bi1 Bi2]. subst.
-    left. eauto.
-  + destruct Bi as [Bi1 Bi2].
-    unfold subenv in H. specialize (H xb Tb Bi2). destruct H as [Bi' | Bi'].
-    * left. eauto.
-    * right. destruct Bi' as [T' [Bi1' Bi2']].
-      exists T'. split. eauto. apply weaken_subtyp. assumption. eauto.
+  intros. induction H; intros; auto.
 Qed.
+Hint Resolve subenv_push.
+
 
 (** [G ⊢ S <: U]                      #<br>#
     [ok(G, x: S)] (see [subenv_push]) #<br>#
@@ -50,13 +57,26 @@ Qed.
 Lemma subenv_last: forall G x S U,
   G ⊢ S <: U ->
   ok (G & x ~ S) ->
-  subenv (G & x ~ S) (G & x ~ U).
+  (G & x ~ S) ⪯ (G & x ~ U).
 Proof.
-  intros. unfold subenv. intros y T Bi.
-  apply binds_push_inv in Bi. destruct Bi as [Bi | Bi].
-  - destruct Bi. subst. right. exists S. split; eauto using weaken_subtyp.
-  - destruct Bi. left. eauto.
+  intros.
+  inversion H0;
+  match goal with
+  | [ H : empty = _ |- _ ] => destruct (empty_push_inv H2)
+  | [ H : _ & _ ~ _ = _ & _ ~ _ |- _ ] =>
+    apply eq_push_inv in H; destruct_all; subst
+  end;
+  constructor; auto.
 Qed.
+Hint Resolve subenv_last.
+
+
+Lemma subenv_implies_ok : forall G1 G2,
+    G1 ⪯ G2 -> ok G1 /\ ok G2.
+Proof.
+  intros. inversion H; split; auto.
+Qed.
+
 
 (** * Narrowing Lemma *)
 (** The narrowing lemma states that typing is preserved under subenvironments.
@@ -98,36 +118,40 @@ Note: for simplicity, the definition typing judgements and [ok] conditions
       are omitted from the paper formulation. *)
 Lemma narrow_rules:
   (forall G t T, G ⊢ t : T -> forall G',
-    ok G' ->
-    subenv G' G ->
+    G' ⪯ G ->
     G' ⊢ t : T)
 /\ (forall G d D, G /- d : D -> forall G',
-    ok G' ->
-    subenv G' G ->
+    G' ⪯ G ->
     G' /- d : D)
 /\ (forall G ds T, G /- ds :: T -> forall G',
-    ok G' ->
-    subenv G' G ->
+    G' ⪯ G ->
     G' /- ds :: T)
 /\ (forall G S U, G ⊢ S <: U -> forall G',
-    ok G' ->
-    subenv G' G ->
+    G' ⪯ G ->
     G' ⊢ S <: U).
 Proof.
   apply rules_mutind; intros; eauto 4;
-    try solve [fresh_constructor; auto using subenv_push].
+    try solve [
+          match goal with
+          | [ H : _ ⪯ _ |- _ ] => destruct (subenv_implies_ok H)
+          end;
+          fresh_constructor].
+  
   Case "ty_var".
+  induction H; auto;
   match goal with
-  | [ Hs: subenv _ _, Hb: binds ?x ?T _ |- _ ] =>
-    specialize (Hs x T Hb);
-    destruct_all; eauto
-  end.
+  | [ H : binds _ _ (_ & _) |- _ ] =>
+    apply binds_push_inv in H; destruct_all; subst
+  end;
+  [ eapply ty_sub; [eauto 2 | apply weaken_subtyp; trivial]
+  | apply weaken_ty_trm; auto].
 Qed.
+
 
 (** The narrowing lemma, formulated only for term typing. *)
 Lemma narrow_typing: forall G G' t T,
   G ⊢ t : T ->
-  subenv G' G -> ok G' ->
+  G' ⪯ G -> 
   G' ⊢ t : T.
 Proof.
   intros. apply* narrow_rules.
@@ -136,8 +160,26 @@ Qed.
 (** The narrowing lemma, formulated only for subtyping. *)
 Lemma narrow_subtyping: forall G G' S U,
   G ⊢ S <: U ->
-  subenv G' G -> ok G' ->
+  G' ⪯ G -> 
   G' ⊢ S <: U.
 Proof.
   intros. apply* narrow_rules.
 Qed.
+
+
+Lemma subenv_trans : forall G1 G2 G3,
+    G1 ⪯ G2 ->
+    G2 ⪯ G3 ->
+    G1 ⪯ G3.
+Proof.
+  introv H. gen G3. induction H; intros; auto.
+  dependent induction H3.
+  - apply empty_push_inv in x. contradiction.
+  - rename x into He. apply eq_push_inv in He. destruct_all.
+    subst.
+    apply IHsubenv in H3.
+    constructor; auto.
+    apply narrow_subtyping with (G':=G) in H6; auto.
+    eapply subtyp_trans; eauto.
+Qed.
+Hint Resolve subenv_trans.
